Refactoring of Mergesort2.v. Cleanup of PairingSort.v. Defined a generic insertion sort using technique from the thesis. Also tried defining a generic selection sort, but looks like it's way tougher.

Sorting/Mergesort2.v
@@ -1,237 +1,99 @@
-Require Export Coq.Program.Wf.
 Require Export Recdef.
-Require Export Div2.
 
 Require Export Sorting.Sort.
 Require Export ListLemmas.
 
-Class Split {A : Type} (small : list A -> bool) : Type :=
+Class msArgs : Type :=
 {
+    A : Type;
+    small : list A -> bool;
+    adhoc : list A -> list A;
     split : list A -> list A * list A;
+    merge : list A -> list A -> list A;
+
     split_spec_l :
       forall l : list A,
         small l = false -> length (fst (split l)) < length l;
     split_spec_r :
       forall l : list A,
         small l = false -> length (snd (split l)) < length l;
+
+    R : A -> A -> Prop;
+
+    Sorted_adhoc :
+      forall l : list A,
+        small l = true -> Sorted R (adhoc l);
+
+    Sorted_merge :
+      forall l l1 l2 : list A,
+        Sorted R l1 -> Sorted R l2 -> Sorted R (merge l1 l2);
+
+    perm_adhoc :
+      forall l : list A,
+        small l = true -> perm (adhoc l) l;
+
+    perm_split :
+      forall l l1 l2 : list A,
+        split l = (l1, l2) -> perm (l1 ++ l2) l;
+
+    perm_merge :
+      forall l1 l2 : list A,
+        perm (merge l1 l2) (l1 ++ l2);
 }.
 
-Coercion split : Split >-> Funclass.
+Coercion A : msArgs >-> Sortclass.
 
-Function ghms
-  {A : Type}
-  (small : list A -> bool)
-  (adhoc : list A -> list A)
-  (split : Split small)
-  (merge : list A -> list A -> list A)
-  (l : list A) {measure length l} : list A :=
-    if small l
-    then adhoc l
-    else
-      let
-        (l1, l2) := split l
-      in
-        merge (ghms small adhoc split merge l1)
-              (ghms small adhoc split merge l2).
+Function ms (args : msArgs) (l : list A) {measure length l} : list A :=
+  if small l
+  then adhoc l
+  else
+    let
+      (l1, l2) := split l
+    in
+      merge (ms args l1)
+            (ms args l2).
 Proof.
-  intros. replace l2 with (snd (split0 l)).
-    apply split_spec_r. assumption.
-    rewrite teq0. cbn. reflexivity.
-  intros. replace l1 with (fst (split0 l)).
-    apply split_spec_l. assumption.
-    rewrite teq0. cbn. reflexivity.
-Defined.
+  all: intros.
+    apply split_spec_r in teq. rewrite teq0 in teq. cbn in teq. assumption.
+    apply split_spec_l in teq. rewrite teq0 in teq. cbn in teq. assumption.
+Time Defined.
 
-Functional Scheme div2_ind := Induction for div2 Sort Prop.
 
-Lemma div2_lt_S :
-  forall n : nat, div2 n < S n.
+Theorem Sorted_ms :
+  forall (args : msArgs) (l : list A),
+    Sorted R (ms args l).
 Proof.
-  intros. functional induction @div2 n; lia.
+  intros. functional induction ms args l.
+    apply Sorted_adhoc. assumption.
+    apply Sorted_merge; assumption.
 Qed.
 
-(*
-#[refine]
-Instance HalfSplit (A : LinDec) : Split A :=
-{
-    split' l :=
-      let n := div2 (length l) in
-      let l1 := take n l in
-      let l2 := drop n l in (l1, l2)
-}.
+Theorem perm_ms :
+  forall (args : msArgs) (l : list A),
+    perm (ms args l) l.
 Proof.
-  intros. destruct l as [| x [| y t]]; cbn in *.
-    lia.
-    lia.
-    inversion H; subst; cbn. apply lt_n_S. apply take_length_lt. cbn.
-      apply div2_lt_S.
-  intros. inversion H; subst. apply drop_length_lt. cbn.
-    destruct l as [| x [| y t]]; cbn in *; lia.
-    destruct l as [| x [| y t]]; cbn in *; inversion 1. lia.
-  intros. cbn. rewrite take_drop. reflexivity.
-Defined.
-*)
-
-Fixpoint interleave {A : Type} (l1 l2 : list A) : list A :=
-match l1, l2 with
-    | [], _ => l2
-    | _, [] => l1
-    | h1 :: t1, h2 :: t2 => h1 :: h2 :: interleave t1 t2
-end.
-
-Theorem ms_split_interleave :
-  forall (A : Type) (l : list A),
-    interleave (fst (ms_split l)) (snd (ms_split l)) = l.
-Proof.
-  induction l as [| | h h' t] using list_ind2; cbn; auto.
-    destruct (ms_split t). cbn in *. rewrite IHt. auto.
+  intros. functional induction ms args l.
+    apply perm_adhoc. assumption.
+    rewrite perm_merge, <- (perm_split l l1 l2).
+      apply perm_app; assumption.
+      assumption.
 Qed.
 
-Lemma count_interleave :
-  forall (A : Type) (p : A -> bool) (l1 l2 : list A),
-    count p (interleave l1 l2) = count p l1 + count p l2.
+Theorem Permutation_ms :
+  forall (args : msArgs) (l : list A),
+    Permutation (ms args l) l.
 Proof.
-  induction l1 as [| h1 t1]; cbn; auto.
-    destruct l2 as [| h2 t2]; cbn.
-      apply plus_n_O.
-      rewrite IHt1. destruct (p h1), (p h2); lia.
+  intros. apply perm_Permutation, perm_ms.
 Qed.
 
-Lemma perm_interleave :
-  forall (A : LinDec) (l1 l1' l2 l2' : list A),
-    perm l1 l1' -> perm l2 l2' ->
-      perm (interleave l1 l2) (interleave l1' l2').
-Proof.
-  unfold perm. intros. rewrite !count_interleave. auto.
-Qed.
-
-(* TODO: fix Mergesort2
-Lemma merge_perm_interleave :
-  forall (A : LinDec) (l : list A * list A),
-    perm (ghms A l) (interleave (fst l) (snd l)).
-Proof.
-  unfold perm; intros. rewrite count_interleave.
-  rewrite <- merge_perm. rewrite count_app. auto.
-Qed.
 
 #[refine]
-Instance MsSplit (A : LinDec) : Split A :=
+Instance Sort_ghms
+  (args : msArgs) : Sort R :=
 {
-    split' := ms_split;
+    sort := ms args
 }.
 Proof.
-  intros. destruct l as [| x [| y t]]; cbn in *.
-    lia.
-    lia.
-    eapply ms_split_len1. eauto.
-  intros. destruct l as [| x [| y t]]; cbn in *.
-    lia.
-    lia.
-    eapply ms_split_len2. eauto.
-  intros. rewrite <- ms_split_interleave at 1.
-    rewrite <- merge_perm_interleave. rewrite merge_perm. reflexivity.
+  apply Sorted_ms.
+  apply Permutation_ms.
 Defined.
-
-Definition ms (A : LinDec) :=
-  @ghms 0 A (fun l => l) (MsSplit A).
-
-Definition ms2 (A : LinDec) :=
-  @ghms 0 A (fun l => l) (HalfSplit A).
-
-(** Time for ultimate mergesort! *)
-
-Function ums
-  (A : LinDec)
-  (depth : nat) (maxdepth : nat)
-  (sort : list A -> list A)
-  (split : Split A)
-  (l : list A)
-  {measure length l} : list A :=
-    if @leqb natle maxdepth depth
-    then sort l
-    else if @leqb natle (length l) 2
-    then sort l
-    else let (l1, l2) := split l in
-      merge A (@ums A (1 + depth) maxdepth sort split l1,
-               @ums A (1 + depth) maxdepth sort split l2).
-Proof.
-  intros. apply split'_spec2 with l1; dec.
-    cbn in *. lia.
-  intros. apply split'_spec1 with l2; dec.
-    cbn in *. lia.
-Defined.
-
-(** Time for ultimatier mergesort. *)
-
-Class Small (A : LinDec) : Type :=
-{
-    small :> nat -> list A -> bool;
-    small_spec :
-      forall (n : nat) (l : list A),
-        small n l = false -> 2 <= length l;
-(*    small_inr :
-      forall (n : nat) (h : A) (t l : list A),
-         small n l = inr (h, t) -> Permutation l (h :: t)*)
-}.
-
-Coercion small : Small >-> Funclass.
-
-Function ums'
-  (A : LinDec)
-  (recdepth : nat)
-  (s : Small A)
-  (sort : list A -> list A)
-  (split : Split A)
-  (l : list A)
-  {measure length l} : list A :=
-    if small recdepth l
-    then sort l
-    else
-      let
-        (l1, l2) := split l
-      in
-        merge A (ums' (1 + recdepth) s sort split l1,
-                 ums' (1 + recdepth) s sort split l2).
-Proof.
-  intros. apply split'_spec2 with l1.
-    assumption.
-    eapply small_spec. eassumption.
-  intros. apply split'_spec1 with l2.
-    assumption.
-    eapply small_spec. eassumption.
-Defined.
-
-Definition ums_wut A := @ums' A 0.
-
-#[refine]
-Instance Small_recdepth (A : LinDec) (max : nat) : Small A :=
-{
-    small recdepth l :=
-      match l with
-          | [] | [_] => true
-          | _ => @leqb natle max recdepth
-      end
-}.
-Proof.
-  destruct l as [| x [| y t]]; cbn.
-    1-2: inv 1.
-    dec.
-Defined.
-
-Function trollms
-  (A : LinDec)
-  (fuel : nat)
-  (sort : list A -> list A)
-  (split : Split A)
-  (l : list A)
-  : list A :=
-match fuel with
-    | 0 => sort l
-    | S fuel' =>
-        let
-          (l1, l2) := split l
-        in
-          merge A (trollms fuel' sort split l1,
-                   trollms fuel' sort split l2)
-end.
-*)
