Sorting/PairingSort.v
@@ -5,48 +5,48 @@ Require Export PairingHeap.
 
 Set Implicit Arguments.
 
-(*Fixpoint sum (l : list nat) : nat :=
+Fixpoint sum (l : list nat) : nat :=
 match l with
     | [] => 0
     | n :: ns => n + sum ns
 end.
 
-Fixpoint size {A : LinDec} (h : PairingHeap A) : nat :=
+Fixpoint size {A : Type} (h : PairingHeap A) : nat :=
 match h with
     | E => 0
     | T _ l => S (sum (map size l))
 end.
 
 Lemma size_empty :
-  forall A : LinDec, size empty = 0.
+  forall A : Type, size (@empty A) = 0.
 Proof. reflexivity. Qed.
 
 Lemma size_singleton :
-  forall (A : LinDec) (x : A), size (singleton x) = 1.
+  forall (A : Type) (x : A), size (singleton x) = 1.
 Proof. reflexivity. Qed.
 
 Lemma size_merge :
-  forall (A : LinDec) (h1 h2 : PairingHeap A),
-    size (merge h1 h2) = size h1 + size h2.
+  forall (A : Type) (p : A -> A -> bool) (h1 h2 : PairingHeap A),
+    size (merge p h1 h2) = size h1 + size h2.
 Proof.
   induction h1 using Tree_ind_proper.
     reflexivity.
-    destruct h2; dec.
+    destruct h2; cbn; try destruct (p x a); cbn; lia.
 Qed.
 
 Lemma size_insert :
-  forall (A : LinDec) (x : A) (h : PairingHeap A),
-    size (insert x h) = S (size h).
+  forall (A : Type) (p : A -> A -> bool) (x : A) (h : PairingHeap A),
+    size (insert p x h) = S (size h).
 Proof.
   intros. apply size_merge.
 Qed.
 
 Lemma size_mergePairs :
-  forall (A : LinDec) (l : list (Tree A)),
-    size (mergePairs l) = sum (map size l).
+  forall (A : Type) (p : A -> A -> bool) (l : list (Tree A)),
+    size (mergePairs p l) = sum (map size l).
 Proof.
-  intros. functional induction mergePairs l; cbn.
-    trivial.
-    rewrite <- plus_n_O. trivial.
-    rewrite !size_merge, IHp, plus_assoc. trivial.
-Qed.*)
+  intros. functional induction mergePairs p l; cbn.
+    reflexivity.
+    rewrite <- plus_n_O. reflexivity.
+    rewrite !size_merge, IHp0, plus_assoc. reflexivity.
+Qed.
