Sorting/GeneralizedInsertionSort.v
@@ -1,0 +1,62 @@
+Require Import List.
+Import ListNotations.
+
+Require Export Sorting.Sort.
+
+Set Implicit Arguments.
+
+Class ISArgs : Type :=
+{
+    A : Type;
+    S : Type;
+
+    empty  : S;
+    insert : A -> S -> S;
+
+    toList : S -> list A;
+
+    R : A -> A -> Prop;
+
+    Sorted_toList :
+      forall s : S, Sorted R (toList s);
+
+    countS : (A -> bool) -> S -> nat;
+
+    countS_empty :
+      forall p : A -> bool,
+        countS p empty = 0;
+
+    countS_insert :
+      forall (p : A -> bool) (x : A) (s : S),
+        countS p (insert x s) = if p x then 1 + countS p s else countS p s;
+
+    countS_toList :
+      forall (p : A -> bool) (s : S),
+        countS p s = count p (toList s);
+}.
+
+Fixpoint fromList (args : ISArgs) (l : list A) : S :=
+match l with
+    | [] => empty
+    | h :: t => insert h (fromList args t)
+end.
+
+Definition insSort (args : ISArgs) (l : list A) : list A := toList (fromList args l).
+
+Lemma countS_fromList :
+  forall (args : ISArgs) (p : A -> bool) (l : list A),
+    countS p (fromList args l) = count p l.
+Proof.
+  induction l as [| h t]; cbn.
+    rewrite countS_empty. reflexivity.
+    rewrite countS_insert, IHt. reflexivity.
+Qed.
+
+Lemma perm_insSort :
+  forall (args : ISArgs) (l : list A),
+    perm (insSort args l) l.
+Proof.
+  unfold perm, insSort. intros.
+  rewrite <- countS_toList, <- countS_fromList.
+  reflexivity.
+Qed.
