Sorting/GeneralizedSelectionSort.v
@@ -1,0 +1,69 @@
+Require Import List.
+Import ListNotations.
+
+Require Export Sorting.Sort.
+
+Set Implicit Arguments.
+
+Class ssArgs : Type :=
+{
+    A : Type;
+    S : Type;
+
+    fromList : list A -> S;
+
+    extractMin : S -> option (A * S);
+
+    size : S -> nat;
+
+    size_extractMin :
+      forall (a : A) (s s' : S),
+        extractMin s = Some (a, s') -> size s' < size s;
+
+    R : A -> A -> Prop;
+
+(*     Sorted_extractMin :
+      forall (a : A) (s s' : S),
+        extractMin s = Some (a, s') -> 
+ *)
+    countS : (A -> bool) -> S -> nat;
+
+    countS_fromList :
+      forall (p : A -> bool) (l : list A),
+        countS p (fromList l) = count p l;
+}.
+
+Function toList (args : ssArgs) (s : S) {measure size s} : list A :=
+match extractMin s with
+    | None => []
+    | Some (h, s') => h :: toList args s'
+end.
+Proof.
+  intros. eapply size_extractMin. eassumption.
+Defined.
+
+Definition ss (args : ssArgs) (l : list A) : list A := toList args (fromList l).
+
+Lemma Sorted_ss :
+  forall (args : ssArgs) (l : list A),
+    Sorted R (ss args l).
+Proof.
+  unfold ss. intros. generalize (fromList l). intros.
+  functional induction toList args s.
+    constructor.
+Abort.
+
+Lemma perm_ss :
+  forall (args : ssArgs) (l : list A),
+    perm (ss args l) l.
+Proof.
+  unfold perm, ss. intros.
+  generalize (fromList l). intros. revert l.
+  functional induction (toList args s); cbn; intros.
+    admit.
+    destruct (p h) eqn: Hph.
+      rewrite (IHl (h :: l)). cbn. rewrite Hph.
+    rewrite IHl.  
+  rewrite <- countS_toList, <- countS_fromList.
+  reflexivity.
+Qed.
